proofs/DSigmaHCOL/ReifyDSHCOL.v
@@ -895,19 +895,46 @@ Proof.
     + compute; reflexivity.
   -
     simpl.
-    unfold evalDSHInductor.
-    HERE: looks like we need to repace in function as well. since gamma changed
-    pose proof (NExpr_NVar_subst_S_head (σ++Γ) n j) as H.
+    pose proof (NExpr_NVar_subst_S_head (σ++Γ) n j) as Hn.
     repeat break_match;crush; try some_none_contradiction; try some_inv; try congruence.
-    f_equiv.
-    f_equiv.
-    repeat nat_equiv_to_eq; subst.
-    apply Some_inj_equiv.
-    rewrite <- Heqo0, <- Heqo2; clear Heqo0 Heqo2.
-
-
-    replace l0 with l by apply proof_irrelevance.
-    reflexivity.
+    +
+      f_equiv.
+      f_equiv.
+      repeat nat_equiv_to_eq; subst.
+      apply Some_inj_equiv.
+      rewrite <- Heqo0, <- Heqo2; clear Heqo0 Heqo2 c c0.
+      generalize (Vhead y). intros y'. clear y. rename y' into y.
+      clear Heqo Heqo1.
+      induction n1.
+      * reflexivity.
+      *
+        rewrite 2!evalDSHInductor_Sn.
+        Opaque evalDSHInductor. simpl.
+        repeat break_match; try reflexivity.
+        unfold evalBinCarrierA.
+        apply AExpr_NVar_subst_S with (j:=j).
+        Transparent evalDSHInductor.
+        --
+          intros pos H.
+          destruct pos; crush.
+          destruct pos; crush.
+          some_inv.
+          f_equiv.
+          constructor.
+          symmetry.
+          apply IHn1.
+          destruct pos; crush.
+        -- compute; reflexivity.
+        -- compute; reflexivity.
+        -- some_none_contradiction.
+        -- some_none_contradiction.
+    +
+      exfalso.
+      admit.
+    +
+      exfalso.
+      admit.
+  -
 Admitted.
 
 Theorem IReduction_DSHIReduction
